

$$f(x) = \prod_{j=a}^b \text{term}(x, j)$$

1. Term Evaluation

$$\alpha(x, i) = \frac{\text{term}(x, i)}{\text{term}(x, i-1)} \quad ;$$

if α holds true for all j

```
- term = term(x, a); f = term;
  for (i=a+1; i<=b; i++) {
    term *=  $\alpha(x, i)$ ;
    f += term;
  }
```

2. Horner's Method

$$f(x, b) = 1 + g(x, b) * f(x, b-1) \quad (f(a) = \text{value})$$

$$f = f(a);$$

```
for (i=a+1; i<=b; i++) {
  f = 1 +  $g(x, i)$  * f ;
}
```

- Horner's Method Accumulates less approximation, round off errors and is more resistant to overflow & underflow errors.
- Term Evaluation can be halted anytime without going to n^{th} term, while Horner's method HAS to go to n^{th} term.

$$\begin{aligned}
 1. \quad f(r, N) &= 1 + r + r^2 + r^3 + \dots + r^{N-2} + r^{N-1} \\
 &= 1 + r(1 + r + r^2 + \dots + r^{N-3} + r^{N-2})
 \end{aligned}$$

$$f(r, N) = 1 + r \times f(r, N-1)$$

$$\alpha = r$$

$$f(r, 0) = 1$$

$$2. \quad f(x, a, N) = \sum_{k=0}^a \frac{x^k}{k!} \left(\prod_{j=0}^{k-1} (a-j) \right)$$

$$= 1 + xa + \frac{x^2}{2} a(a-1) + \frac{x^3}{2 \cdot 3} a(a-1)(a-2) + \dots$$

$$= 1 + xa \left(1 + \frac{x(a-1)}{2} + \frac{x^2(a-1)(a-2)}{2 \cdot 3} + \frac{x^3(a-1)(a-2)(a-3)}{2 \cdot 3 \cdot 4} + \dots \right)$$

$$= 1 + xa \left(1 + \frac{x(a-1)}{2} \left(1 + \frac{x}{3} (a-2) + \frac{x^2(a-2)(a-3)}{3 \cdot 4} + \dots \right) \right)$$

$$f(x, a, T) = 1 + \frac{x(a-T)}{(1+T)} f(x, a, T+1) \quad (T_0 = 0)$$

$$f(x, a, N-1) = 1 \quad (T_0 \text{ stop at } N^{\text{th}} \text{ term})$$

$$\text{Or } \alpha = \text{term}(k) \div \text{term}(k-1)$$

$$\frac{x^k}{k!} \prod_{j=0}^{k-1} (\alpha - j) \div \frac{x^{k-1}}{(k-1)!} \prod_{j=0}^{k-2} (\alpha - j)$$

$$\Rightarrow \frac{x}{k} (\alpha - k + 1) \frac{x^{k-1}}{(k-1)!} \prod_{j=0}^{k-2} (\alpha - j) \div \frac{x^{k-1}}{(k-1)!} \prod_{j=0}^{k-2} (\alpha - j) = 1$$

$$\alpha = \frac{x}{k} (\alpha - k + 1)$$

$$3. J(x) = \sum_{K=0}^{\infty} \frac{(-1)^K}{(K!)^2} \left(\frac{x}{2}\right)^{2K}$$

$$= 1 + \sum_{K=1}^{\infty} \frac{(-1)^K}{(K!)^2} \left(\frac{x}{2}\right)^{2K}$$

$$= 1 - \frac{x^2}{2^2} + \frac{x^4}{2^4} \frac{1}{(2!)^2} - \frac{x^6}{2^6} \frac{1}{(3 \cdot 2)^2} - \dots$$

$$= 1 - \frac{x^2}{2^2} \left(1 - \frac{x^2}{2^2} \frac{1}{2^2} + \frac{x^4}{2^4} \frac{1}{(3 \cdot 2)^2} - \frac{x^6}{2^6} \frac{1}{(4 \cdot 3 \cdot 2)^2} - \dots \right)$$

$$= 1 - \frac{x^2}{2^2} \left(1 - \frac{x^2}{2^2} \frac{1}{2^2} \left(1 - \frac{x^2}{2^2} \frac{1}{3^2} + \frac{x^4}{2^4} \frac{1}{(4 \cdot 3)^2} - \dots \right) \right)$$

$$J(x, t, N) = 1 - \frac{x^2}{2^2} \frac{1}{t^2} J(x, t+1, N)$$

$$J(x, N, N) = 1$$

$$\alpha = \frac{(-1)^K}{(K!)^2} \left(\frac{x}{2}\right)^{2K} \times \frac{((K-1)!)^2}{(-1)^{K-1}} \left(\frac{x}{2}\right)^{2(K-1)}$$

$$\alpha = -\frac{1}{K^2} \cdot \left(\frac{x}{2}\right)^2$$

4.

$$f(s) = \sum_{n=1}^{\infty} \frac{1}{n^s}$$

$$f(s) = 1^{-s} + 2^{-s} + 3^{-s} + \dots$$

$$n^s = t$$

$$\log n^s = \log t$$

$$s \log n = \log t$$

$$\Rightarrow t = e^{s \cdot \log n}$$

$$5. p(x) = \frac{2}{\sqrt{\pi}} \left(x - \frac{x^3}{3} + \frac{x^5}{10} - \dots \right)$$

$$= \frac{2}{\sqrt{\pi}} \sum_{n=0}^{\infty} \frac{(-1)^n x^{2n+1}}{(2n+1) n!}$$

$$\alpha = \frac{(-1)^n}{(-1)^{n-1}} \frac{2n-1}{2n+1} \frac{(n-1)!}{n!} \frac{x^{2n+1}}{x^{2n-1}}$$

$$\alpha = -\left(\frac{2n-1}{2n+1}\right) \frac{x^2}{n}$$

$$f(x, a, N, T) = 1 + \frac{x(a-T)}{(1+T)} f(x, a, N, T+1) \quad \begin{matrix} T \leq N \\ T=N=1 \end{matrix}$$

$$f(x, a, N) = \sum_{k=0}^a \frac{x^k}{k!} \left(\prod_{j=0}^{k-1} (a-j) \right)$$

$$t(k) = \frac{x^k}{k!} \prod_{j=0}^{k-1} (a-j)$$

$$\frac{t(k+1)}{t(k)} = \frac{x}{k+1} \frac{1}{a-k}$$

$$\text{term} = \frac{x}{(k+1)(a-k)}$$